some memory verification in the cryptobox example

examples/crypto/cryptobox/Box.AE.fst
@@ -2,8 +2,8 @@ module Box.AE
 
 open FStar.Seq
 open FStar.Monotonic.Seq
-open FStar.HyperHeap
 open FStar.HyperStack
+open FStar.HyperHeap
 open FStar.Monotonic.RRef
 
 open Box.Flags
@@ -13,7 +13,10 @@ open Platform.Bytes
 open CoreCrypto
 
 module B = Platform.Bytes
-
+module MR = FStar.Monotonic.RRef
+module HH = FStar.HyperHeap
+module HS = FStar.HyperStack
+module MM = MonotoneMap
 open Box.PlainAE
 
 
@@ -22,16 +25,35 @@ let ivsize = aeadRealIVSize AES_128_GCM
 type keysize = aeadKeySize AES_128_GCM
 type aes_key = lbytes keysize (* = b:bytes{B.length b = keysize} *)
 type cipher = b:bytes{B.length b >= ivsize}
+type nonce = bytes
 (* MK: minimal cipher length twice blocksize? *)
 
-type log_t (i:ae_id) (r:rid) = m_rref r (seq ((protected_ae_plain i) * cipher)) grows
+let ae_region_color = -1
+
+
+private val ae_key_region: (r:MR.rid{extends r root /\ is_eternal_region r /\ (color r = ae_region_color) /\ is_below r root /\ disjoint r id_table_region})
+private let ae_key_region = 
+  recall_region id_table_region;
+  new_colored_region root ae_region_color
+
+
+type log_entry i = (protected_ae_plain i) * cipher * nonce
+type log_t (i:ae_id) (r:rid) = m_rref r (seq (log_entry i)) grows
+
+//type log_key = (cipher * nonce)
+//type log_t (i:ae_id) = MM.t #ae_key_region 
+
+
+val fresh_nonce: #(i:ae_id) -> (n:nonce) -> seq (log_entry i) -> Tot bool
+let fresh_nonce #i n entries =
+  not (Some? (seq_find (fun (_,_,n') -> n' = n) entries))
 
 (**
    The key type is abstract and can only be accessed via the leak and coerce_key functions.
 *)
 
-noeq abstract type key =
-  | Key: #i:ae_id -> #region:rid -> raw:aes_key -> log:log_t i region -> key
+noeq type key =
+  | Key: #i:ae_id -> #(region:rid{extends region ae_key_region}) -> raw:aes_key -> log:log_t i region -> key
 
 val get_index: k:key -> Tot (i:ae_id{i=k.i})
 let get_index k = k.i
@@ -42,32 +64,38 @@ let get_index k = k.i
     Also, it makes sure that the log created along with the key is empty.
 *)
 let safe_key_gen parent m0 k m1 =
-    modifies Set.empty m0 m1
+  // Reason about regions (HyperHeap)
+  HH.modifies Set.empty m0.h m1.h
   /\ extends k.region parent
   /\ fresh_region k.region m0.h m1.h
+  /\ color k.region = ae_region_color
+  /\ is_below k.region ae_key_region
+  // Reason about memory (HyperStack)
   /\ m_contains k.log m1
   /\ m_sel m1 k.log == createEmpty
+
 
 (**
    This function generates a key in a fresh region of memory below the parent region.
    The postcondition ensures that the log is empty after creation.
 *)
-val keygen: i:ae_id -> parent:rid -> ST (k:key{k.i=i})
+val keygen: i:ae_id -> ST (k:key{k.i=i})
   (requires (fun _ -> True))
   (ensures  (fun h0 k h1 -> 
-    safe_key_gen parent h0 k h1
+    safe_key_gen ae_key_region h0 k h1
   ))
-let keygen i parent =
+let keygen i =
   let rnd_k = random keysize in
-  let region = new_region parent in
+  let region = new_colored_region ae_key_region ae_region_color in
   let log = alloc_mref_seq region createEmpty in
   Key #i #region rnd_k log
+
 
 (**
    The leak_key function transforms an abstract key into a raw aes_key.
    The refinement type on the key makes sure that no honest keys can be leaked.
 *)
-val leak_key: k:key{~(ae_honest k.i) \/ ~(b2t ae_ind_cca)} -> Tot aes_key 
+val leak_key: k:key{(ae_dishonest k.i) \/ ~(b2t ae_ind_cca)} -> Tot aes_key 
 let leak_key k =
   k.raw
 
@@ -76,19 +104,25 @@ let leak_key k =
    as we need to allocate space in memory for the key. The refinement type on the key makes sure that
    abstract keys created this way can not be honest.
 *)
-val coerce_key: i:ae_id{(ae_dishonest i) \/ ~(prf_odh)} -> parent:rid -> aes_key -> ST (k:key{k.i=i})
+val coerce_key: i:ae_id{(ae_dishonest i) \/ ~(prf_odh)} -> aes_key -> ST (k:key{k.i=i})
   (requires (fun _ -> True))
-  (ensures  (safe_key_gen parent))
-let coerce_key i parent raw = 
-  let region = new_region parent in
+  (ensures  (safe_key_gen ae_key_region))
+let coerce_key i raw = 
+  let region = new_colored_region ae_key_region ae_region_color in
   let log = alloc_mref_seq region createEmpty in
   Key #i #region raw log
+
 
 (**
    safe_log_append makes sure that new entries added to the log are appended in a memory-safe way.
 *)
-type safe_log_append k entry h0 h1 =
-    modifies_one k.region h0 h1 
+
+//Ideally use this instead of every postcondition separately.
+let safe_log_append k entry h0 h1 =
+    let s1 = Set.singleton id_table_region in
+    let s2 = Set.singleton k.region in
+    let s = Set.union s1 s2 in
+    modifies_just s h0.h h1.h
     /\ m_contains k.log h1
     /\ m_sel h1 k.log == snoc (m_sel h0 k.log) entry
     /\ witnessed (at_least (Seq.length (m_sel h0 k.log)) entry k.log)
@@ -97,48 +131,83 @@ type safe_log_append k entry h0 h1 =
 (**
    Encrypt a a message under a key. Idealize if the key is honest and ae_ind_cca true.
 *)
-val encrypt: #(i:ae_id) -> k:key{k.i=i} -> (m:protected_ae_plain i) -> ST cipher
-  (requires (fun h0 -> True
-    (*m_contains k.log h0*)))
-  (ensures  (fun h0 c h1 -> True 
-//    /\ safe_log_append k (m,c) h0 h1 //add back once memory separation is fixed
+val encrypt: #(i:ae_id) -> n:nonce -> k:key{k.i=i} -> (m:protected_ae_plain i) -> ST cipher
+  (requires (fun h0 -> 
+    let entries = m_sel h0 k.log in
+    fresh_nonce n entries
+  ))
+  (ensures  (fun h0 c h1 ->
+    let s1 = Set.singleton id_table_region in
+    let s2 = Set.singleton k.region in
+    let s = Set.union s1 s2 in
+    modifies_just s h0.h h1.h
+    /\ m_contains k.log h1
+    /\ m_sel h1 k.log == snoc (m_sel h0 k.log) (m,c,n)
+    /\ witnessed (at_least (Seq.length (m_sel h0 k.log)) (m,c,n) k.log)
     ))
-let encrypt #i k m =
+let encrypt #i n k m =
+  admit(); // REMOVE THIS!!!
   m_recall k.log;
   let iv = random ivsize in
-  //assert(ae_dishonest i \/ ae_honest i);
   let ae_honest_i = ae_honestST i in
   let p = if (ae_ind_cca && ae_honest_i) then createBytes (length m) 0z else (repr m) in
   let c = CoreCrypto.aead_encrypt AES_128_GCM k.raw iv empty_bytes p in
   let c = iv@|c in
-  write_at_end k.log (m,c);
+  write_at_end k.log (m,c,n);
   c
 
+
+val is_in_entries: #i:ae_id -> log_entry i -> seq (log_entry i) -> Type0
+let is_in_entries #i entry entries =
+  Seq.contains entries entry
+  
 
 (**
    Decrypt a ciphertext c using a key k. If the key is honest and ae_int_ctxt is idealized,
    try to obtain the ciphertext from the log. Else decrypt via concrete implementation.
    TODO: Make this a total function.
 *)
-val decrypt: #(i:ae_id) -> k:key{k.i=i} -> c:cipher -> ST (option (protected_ae_plain i))
-  (requires (fun h -> True (* Could require Map.contains h0 k.region *)))
-  (ensures  (fun h0 res h1 -> True))
-    (* Modifies_none h0 h1 *)
-    (* /\ ( ( ae_ind_cca /\(ae_honest i)) ==> (get_index res) *)
-    (* /\ ( (b2t ae_int_ctxt /\ honest i /\ Some? res) ==> Seq.mem (Some?.v res,c) (m_sel h0 k.log)  *)
-    (* ))) *)
-let decrypt #i k c =
+val decrypt: #(i:ae_id) -> n:nonce -> k:key{k.i=i} -> c:cipher -> ST (option (protected_ae_plain i))
+  (requires (fun h -> Map.contains h.h k.region))
+  (ensures  (fun h0 res h1 -> 
+    modifies_one id_table_region h0.h h1.h
+    /\ ( (~(b2t ae_ind_cca) \/ ae_dishonest i) \/ ((b2t ae_ind_cca /\ ae_honest i /\ Some? res) ==> (is_in_entries (Some?.v res,c,n) (m_sel h0 k.log))))
+    //Some? (seq_find (fun (res',c',n') -> c' = c && n' = n && res' = res) (m_sel h0 k.log)))
+//      Seq.contains (Some?.v res,c,n) (m_sel h0 k.log))
+    ))
+
+//val find_in_entries: #i:ae_id -> log_entry i -> seq (log_entry i) -> Type0
+//let find_in_entries #i entry entries =
+  
+
+let decrypt #i n k c =
+  admit(); //REMOVE THIS !!! (You may have to find proper settings for Z3,
+	   // but this has verified before.
   let ae_honest_i = ae_honestST i in
-  if ae_ind_cca && ae_honest_i then
+  if ae_ind_cca && ae_honest_i then (
     let log = m_read k.log in
-    match seq_find (fun mc -> snd mc = c) log with
-    | Some mc -> Some (fst mc)
+    match Seq.find_l (fun (_,c',n') -> c' = c && n' = n) log with
+    | Some (m,_,_) ->
+      lemma_find_l_contains (fun (_,c',n') -> c' = c && n' = n) log;
+      Some m
     | None -> None
-  else
+  ) else (
     let iv,c' = split c ivsize in
     assume( B.length c' >= aeadTagSize AES_128_GCM);
     let poption = (CoreCrypto.aead_decrypt AES_128_GCM k.raw iv empty_bytes c') in
-//    admit ();
     match poption with
     | Some p -> Some (PlainAE.coerce #i (p))
     | None -> None
+  )
+
+//val dec_enc_inverse_lemma: #(i:ae_id) -> n:nonce -> k:key -> c:cipher -> ST bool
+//  (requires (fun h0 -> 
+//    k.i==i
+//    /\ Map.contains h0.h k.region
+//  ))
+//  (ensures (fun h0 b h1 -> b))
+//let dec_enc_inverse_lemma #i n k c =
+//  match decrypt #i n k c with
+//  | Some m' -> c = encrypt #i n k m'
+//  | None -> true
+    
