examples/crypto/cryptobox/Box.DH.fst
@@ -22,40 +22,28 @@ module MR = FStar.Monotonic.RRef
 module MM = MonotoneMap
 
 
-assume val dh_share_size : nat
+assume val dh_element_size : nat
 assume val dh_exponent_size : nat
-type dh_share = lbytes dh_share_size
+type dh_element =lbytes dh_element_size
+type dh_share = dh_element
+assume val dh_base : dh_element
 abstract type dh_exponent = lbytes dh_exponent_size
 
 assume val dh_gen_key: unit -> St (dh_share*dh_exponent)
 
 type keysize = aeadKeySize AES_128_GCM
 type aes_key = lbytes keysize (* = b:bytes{B.length b = keysize} *)
-
-
-//noeq type entry (i:id) = 
-//  | DH_entry: ent_i:id -> ent_share:dh_share -> ent_key:PlainDH.key{AE.get_index ent_key = (i,ent_i) /\ ae_honest (i,ent_i)} -> entry i
-
+assume val hash: dh_element -> aes_key
 
 (*
   Setting up a global log for AE.keys indexed by the ids of the public and private key involved.
 *)
-private type range = fun (k_id:ae_id) -> k:PlainDH.key{(AE.get_index k = k_id) || (AE.get_index k = (snd k_id,fst k_id))}
+private type range = fun (k_id:ae_id) -> k:PlainDH.key{PlainDH.ae_key_get_index k = k_id}
 private let inv (f:MM.map' (ae_id) range) = True
-//type log_t (i:id) (r:rid) = m_rref r (seq (entry i)) grows
 private let ae_key_log = MM.alloc #root #ae_id #range #inv
-private let (ae_key_region:MR.rid) = new_region root
 
-
-//noeq abstract type dh_pkey = 
-//  | DH_pkey:  #pk_id:id -> #region:rid ->rawpk:dh_share -> log:log_t pk_id region -> dh_pkey
-//
-//
-//noeq abstract type dh_skey =
-//  | DH_skey: #sk_id:id -> rawsk:dh_exponent -> pk:dh_pkey{pk.pk_id=sk_id} -> dh_skey 
 noeq abstract type dh_pkey = 
   | DH_pkey:  #pk_id:id -> rawpk:dh_share -> dh_pkey
-
 
 noeq abstract type dh_skey =
   | DH_skey: #sk_id:id -> rawsk:dh_exponent -> pk:dh_pkey{pk.pk_id=sk_id} -> dh_skey 
@@ -70,38 +58,28 @@ val pk_get_rawpk: pk:dh_pkey -> Tot (raw:dh_share{raw=pk.rawpk})
 let pk_get_rawpk pk =
   pk.rawpk
 
+assume val dh_exponentiate: dh_element -> dh_exponent -> Tot dh_element
+
 val keygen: #i:id -> ST (dh_pair:(k:dh_pkey{k.pk_id=i}) * (k:dh_skey{k.sk_id=i}))
   (requires (fun h -> True))
-  (ensures (fun h0 k h1 -> True
-//  let (pk,sk) = k in
-//  safe_key_gen parent pk h0 h1
-  ))
+  (ensures (fun h0 k h1 -> True))
 let keygen #i =
   let dh_share,dh_exponent = dh_gen_key() in
   let dh_pk = DH_pkey #i dh_share in
   let dh_sk = DH_skey #i dh_exponent dh_pk in
   dh_pk,dh_sk
 
-(**
-   This function takes a dh_share to the power of a dh_exponent.
-   TODO: Actually link to functional code in CoreCrypto?
-*)
-assume val dh_exponentiate: dh_share -> dh_exponent -> Tot aes_key
+val coerce_pkey: #i:id{dishonest i} -> dh_share -> St (pk:dh_pkey{pk.pk_id=i})
+let coerce_pkey #i dh_sh =
+  DH_pkey #i dh_sh
 
-//type safe_log_append pk entry h0 h1 =
-//    modifies_one pk.region h0 h1 
-//    /\ m_contains pk.log h1
-//    /\ m_sel h1 pk.log == snoc (m_sel h0 pk.log) entry
-//    /\ witnessed (at_least (Seq.length (m_sel h0 pk.log)) entry pk.log)
+val coerce_keypair: #i:id{dishonest i} -> dh_exponent -> St (dh_pair:(k:dh_pkey{k.pk_id=i}) * (k:dh_skey{k.sk_id=i}))
+let coerce_keypair #i dh_ex =
+  let dh_sh = dh_exponentiate dh_base dh_ex in
+  let pk = DH_pkey #i dh_sh in
+  let sk = DH_skey #i dh_ex pk in
+  pk,sk
 
-(**
-   Helper function to look entries up in a log.
-*)
-
-//val equal_share: sk_id:id -> pk_id:id -> dh_sh:dh_share -> e:entry sk_id -> Tot bool
-//let equal_share sk_id pk_id dh_sh e =
-//  match e with 
-//  | DH_entry ent_i ent_share _ -> ent_i=pk_id && ent_share = dh_sh
 
 (**
    If we prf_odh is true, the output of this function is random, if both 
@@ -110,12 +88,12 @@ assume val dh_exponentiate: dh_share -> dh_exponent -> Tot aes_key
 val prf_odh: sk:dh_skey -> pk:dh_pkey -> ST (PlainDH.key)
   ( requires (fun _ -> True))
   ( ensures (fun _ k _ -> 
-    (Box.AE.get_index k = (sk.sk_id, pk.pk_id)) || (Box.AE.get_index k = (pk.pk_id, sk.sk_id))
+    (PlainDH.ae_key_get_index k = generate_ae_id sk.sk_id pk.pk_id)
   ))
 let prf_odh dh_sk dh_pk =
   let pk_id = dh_pk.pk_id in
   let sk_id = dh_sk.sk_id in
-  let i = pk_id, sk_id in
+  let i = generate_ae_id pk_id sk_id in
   let ae_honest_i = ae_honestST i in
   if ae_honest_i && prf_odh then
     (MR.m_recall ae_key_log;
@@ -123,34 +101,11 @@ let prf_odh dh_sk dh_pk =
     match entry with
     | Some  k' -> k'
     | None -> 
-      let k' = PlainDH.keygen i ae_key_region in
+      let k' = PlainDH.keygen i in
       MM.extend ae_key_log i k';
       k')
   else
-    let real_k = dh_exponentiate dh_pk.rawpk dh_sk.rawsk in
-    let k=PlainDH.coerce_key i ae_key_region real_k in
+    let raw_k = dh_exponentiate dh_pk.rawpk dh_sk.rawsk in
+    let hashed_raw_k = hash raw_k in
+    let k=PlainDH.coerce_key i hashed_raw_k in
     k
-
-
-
-//val prf_odh_rcv: #(sk_id:id) -> dh_sk:dh_skey{dh_sk.sk_id=sk_id} -> #(pk_id:id) -> dh_snd_pk:dh_pkey{dh_snd_pk.pk_id=pk_id} ->  St (k:PlainDH.key{AE.get_index k = (sk_id,pk_id)}
-//)
-//let prf_odh_rcv #sk_id dh_rcv_sk #pk_id dh_snd_pk  =
-//  let honest_i = ae_honestST (sk_id, pk_id) in
-//  if honest_i && prf_odh then
-//    let log = m_read dh_rcv_sk.pk.log in
-//    let e = seq_find (equal_share sk_id pk_id dh_snd_pk.rawpk) log in
-//    match e with
-//    | Some (DH_entry _ _ k') -> k'
-//    | None -> 
-//      let i = sk_id,pk_id in
-//      let k = PlainDH.keygen i dh_rcv_sk.pk.region in
-//      k
-////      let i = sk_id,dishonestId() in
-////      let raw_k = dh_exponentiate dh_snd_pk.rawpk dh_rcv_sk.rawsk in
-////      admit ();
-////      PlainDH.coerce_key i dh_rcv_sk.pk.region raw_k
-//  else
-//    let i =  sk_id,pk_id in
-//    let raw_k = dh_exponentiate dh_snd_pk.rawpk dh_rcv_sk.rawsk in
-//    PlainDH.coerce_key i dh_rcv_sk.pk.region raw_k
