examples/crypto/cryptobox/Box.Indexing.fst
@@ -9,119 +9,87 @@ module MR = FStar.Monotonic.RRef
 module MM = MonotoneMap
 
 
-// Make these abstract!
-type id = UInt32.t
+// This should be UInt32?
+type id = int
 assume Index_hasEq: hasEq id
-private type range = fun id -> bool
-private let inv (f:MM.map' id range) = True
-private let table = MM.alloc #root #id #range #inv 
+type range = fun id -> bool
+let inv (f:MM.map' id range) = True
+
+let id_table_color = -1
+val id_table_region: (r:MR.rid{color r = id_table_color /\ extends r root /\ is_eternal_region r /\ is_below r root})
+let id_table_region = new_colored_region root id_table_color
+
+
+//val id_table: MM.t
+let id_table = MM.alloc #id_table_region #id #range #inv 
 
 
 //abstract type val honest: i:id -> Tot bool
-let honest (i:id) =
-  MR.witnessed (MM.contains table i true)
+type honest (i:id) =
+  MR.witnessed (MM.contains id_table i true)
 
-let dishonest (i:id) =
-  MR.witnessed (MM.contains table i false)
-
-
-
-val honestST: i:id -> St(b:bool{(b ==> honest i) /\ (not b ==> dishonest i)})
-let honestST (i:id) =
-  MR.m_recall table;
-  match MM.lookup table i with
-  |Some v -> 
-//    MR.testify (MM.contains table i v);
-    v
-  |None -> 
-    MM.extend table i true;
- //   MR.testify (MM.contains table i true);
-    true
+type dishonest (i:id) =
+  MR.witnessed (MM.contains id_table i false)
 
 
-val lemma_hon_implies_not_dis: i:id -> w:(honest i)-> Lemma
-  (requires (True))
-  (ensures (honest i ==> ~(dishonest i)))
-  [SMTPat (honest i)]
-let lemma_hon_implies_not_dis i =
+val make_dishonest: (i:id) -> ST (unit)
+  (requires (fun h0 -> MM.fresh id_table i h0))
+  (ensures (fun h0 _ h1 -> dishonest i))
+let make_dishonest i =
+  MM.extend id_table i false;
   ()
 
+val honestST: i:id -> ST(b:bool{(b ==> honest i) /\ (not b ==> dishonest i)})
+  (requires (fun h0 -> True))
+  (ensures (fun h0 b h1 ->
+    modifies_one id_table_region h0 h1 
+    /\ MR.m_contains id_table h1
+  ))
+let honestST (i:id) =
+  MR.m_recall id_table;
+  match MM.lookup id_table i with
+  |Some v -> 
+    v
+  |None -> 
+    MM.extend id_table i true;
+    true
 
-val lemma_dis_implies_not: i:id -> Lemma 
+abstract type ae_id = 
+  | AE_id: i:(id*id){fst i <= snd i} -> ae_id
+
+val generate_ae_id: i1:id -> i2:id -> Tot (i3:ae_id{fst i3.i <= snd i3.i})
+let generate_ae_id i1 i2 =
+  if i1 <= i2 then
+    AE_id (i1,i2)
+  else
+    AE_id (i2,i1)
+
+val unique_id_generation: i1:id -> i2:id -> Lemma
   (requires (True))
-  (ensures (dishonest i ==> ~(honest i)))
-  [SMTPat (dishonest i) ]
-let lemma_dis_implies_not i = ()
+  (ensures (forall id1 id2. generate_ae_id id1 id2 = generate_ae_id id2 id1))
+  [SMTPat (generate_ae_id i1 i2)]
+let unique_id_generation i1 i2 = ()
 
 
+//val ae_honest: (k_i:ae_id) -> Tot Type0 //(t:Type{t ==> honest (fst k_i.i) /\ honest (snd k_i.i)})
+type ae_honest k_i =
+  honest (fst k_i.i) /\ honest (snd k_i.i)
 
-type ae_id = (id*id)
 
-let ae_honest (i1,i2:ae_id) =
-  MR.witnessed (MM.contains table i1 true) /\
-  MR.witnessed (MM.contains table i2 true)
-  //honest i1 /\ honest i2
+type ae_dishonest (k_i:ae_id) =
+  dishonest (fst k_i.i) \/ dishonest (snd k_i.i)
 
-let ae_dishonest (i1,i2:ae_id) =
-  MR.witnessed (MM.contains table i1 false) \/
-  MR.witnessed (MM.contains table i2 false)
-  //dishonest i1 \/ dishonest i2
-
-val ae_honestST: i:(id*id) -> St(b:bool{(b ==> (ae_honest i)) /\ (not b ==> (ae_dishonest i))})
-let ae_honestST (i1,i2) =
-  let h1 = honestST i1 in 
-  let h2 = honestST i2 in
+val ae_honestST: k_i:ae_id -> ST(b:bool{(b ==> (ae_honest k_i)) /\ (not b ==> (ae_dishonest k_i))})
+  (requires (fun h0 -> True))
+  (ensures (fun h0 b h1 ->
+    modifies_one id_table_region h0 h1 
+    /\ MR.m_contains id_table h1
+    ///\ MR.m_sel h1 id_table == snoc (MR.m_sel h0 id_table) i
+  ))
+let ae_honestST k_i =
+  let h1 = honestST (fst k_i.i) in 
+  let h2 = honestST (snd k_i.i) in
   h1 && h2
 
-val lemma_ae_dis_implies_not: i:ae_id -> Lemma 
-  (requires (True))
-  (ensures (ae_dishonest i ==> ~(ae_honest i)))
-  [SMTPat (ae_honest i) ]
-let lemma_ae_dis_implies_not i = ()
 
-val lemma_ae_hon_implies_not_dis: i:ae_id -> Lemma 
-  (requires (True))
-  (ensures (ae_honest i ==> ~(ae_dishonest i)))
-  [SMTPat (ae_honest i) ]
-let lemma_ae_hon_implies_not_dis i = ()
 
-//private type ae_range = fun (i:ae_id) -> (b:bool{b ==> honest (fst i) /\ honest (snd i)})
-//private let ae_inv (f:MM.map' ae_id ae_range) = True
-//private let ae_table = MM.alloc #root #ae_id #ae_range #ae_inv 
-//
-//
-//
-//assume val generate_ae_id: i1:id -> i2:id -> Tot (i3:ae_id{i3=(i1,i2)})
-//
-//
-////assume val ae_honest: i:ae_id -> Tot (b:bool{b ==> (honest (fst i) /\ honest (snd i))})
-//let ae_honest (i:ae_id) =
-//  honest (fst i) /\ honest (snd i) /\
-//  MR.witnessed (MM.contains ae_table i true)
-//
-//let ae_dishonest (i:ae_id) =
-//  dishonest (fst i) \/ dishonest (snd i) \/
-//  MR.witnessed (MM.contains ae_table i false)
-//
-//assume val lemma_ae_dis_implies_not: i:ae_id -> Lemma 
-//  (requires (True))
-//  (ensures (ae_dishonest i ==> ~(ae_honest i)))
-//  [SMTPat (ae_dishonest i) ]
-//  
-//val ae_honestST: i:ae_id -> ST(b:bool{(b ==> ae_honest i) /\ (not b ==> ae_dishonest i)})
-//  (requires (fun h0 -> True))
-//  (ensures (fun h0 t h1 -> 
-//    modifies (Set.singleton root) h0 h1 // precise enough?
-//    ))
-//let ae_honestST (i:ae_id) =
-//  MR.m_recall ae_table;
-//  match MM.lookup ae_table i with
-//  |Some v -> 
-//    v=true
-//  |None -> 
-//    MM.extend ae_table i false;
-//    false
-//
-//
-////val ae_honest: i:ae_id -> Tot (b:bool ==> (forall x. mem x i ==> honest x))
-//
